src/strtoimax/asn_strtoimax_lim_spec.v
@@ -4,7 +4,7 @@ Import ListNotations.
 Require Import StructTact.StructTactics.
 Require Import IntNotations.
 Require Import asn_strtoimax_lim.
-Local Open Scope IntScope.
+Local Open Scope Int64Scope.
 
 (* Functional specification of INTEGER.c/asn_strtoimax_lim *)
 
@@ -84,7 +84,7 @@ Notation minus_char := (Int.repr 45).
 Notation plus_char := (Int.repr 43).
 Notation zero_char := (Int.repr 48).
 
-Definition ASN1_INTMAX_MAX :=(Int.not 0) >> 1.
+Definition ASN1_INTMAX_MAX :=(Int64.not 0) >> 1.
 
 Fact shift_pow2_div :  (Int64.shru (Int64.not Int64.zero) Int64.one) = Int64.repr (Int64.max_unsigned / 2).
   replace (Int64.not Int64.zero) with (Int64.repr Int64.max_unsigned) by (auto with ints).
@@ -92,17 +92,19 @@ Fact shift_pow2_div :  (Int64.shru (Int64.not Int64.zero) Int64.one) = Int64.rep
   f_equal.
   Qed.
 
-Definition upper_boundary := ASN1_INTMAX_MAX // (Int.repr 10).
-Definition last_digit_max_plus := ASN1_INTMAX_MAX % (Int.repr 10).
-Definition last_digit_max_minus := (ASN1_INTMAX_MAX % (Int.repr 10)) + 1.
+Definition upper_boundary := ASN1_INTMAX_MAX // (Int64.repr 10).
+Definition last_digit_max := ASN1_INTMAX_MAX % (Int64.repr 10).
+Definition last_digit_max_minus := (ASN1_INTMAX_MAX % (Int64.repr 10)) + 1.
 (* [0-9]*)
 Definition digits := map Int.repr [48;49;50;51;52;53;54;55;56;57].
 Definition is_digit (i : int) := existsb (fun j => Int.eq i j) digits.
 Definition distance (a1 a2 : addr) : nat :=
   ((Z.to_nat (Ptrofs.unsigned (snd a2))) - (Z.to_nat (Ptrofs.unsigned (snd a1))))%nat.
 
+Definition int_to_int64 (i : int) := Int64.repr (Int.unsigned i).
+
 (* Functional spec *)
-Fixpoint asn_strtoimax_lim_loop (str : addr) (fin : addr) (value : int) (s: signedness) (last_digit : int) (dist : nat) (m' : mem) {struct dist} : option (asn_strtox_result_e*(option(int*signedness))*(option mem)) :=
+Fixpoint asn_strtoimax_lim_loop (str : addr) (fin : addr) (value : int64) (s: signedness) (last_digit : int64) (dist : nat) (m' : mem) {struct dist} : option (asn_strtox_result_e*(option(int64*signedness))*(option mem)) :=
   let m' := (Mem.storev Mptr m (vptr fin) (vptr str)) in
      match dist with
                 | O => Some (ASN_STRTOX_OK, Some (value, s), m')
@@ -110,8 +112,8 @@ Fixpoint asn_strtoimax_lim_loop (str : addr) (fin : addr) (value : int) (s: sign
                         | Some (Vint i) =>
                           if is_digit i
                           then
-                            let d := i - zero_char in
-                            let v := (value*(Int.repr 10) + d) in
+                            let d := int_to_int64 (i - zero_char)%int in
+                            let v := (value*(Int64.repr 10) + d) in
                             if value < upper_boundary
                             then asn_strtoimax_lim_loop (str++) fin v s last_digit n m
                             else if (value == upper_boundary) && (d <= last_digit)
@@ -122,7 +124,7 @@ Fixpoint asn_strtoimax_lim_loop (str : addr) (fin : addr) (value : int) (s: sign
                         end
   end.
     
-Definition asn_strtoimax_lim (str fin : addr) : option (asn_strtox_result_e*(option(int*signedness))*(option mem)) :=
+Definition asn_strtoimax_lim (str fin : addr) : option (asn_strtox_result_e*(option(int64*signedness))*(option mem)) :=
   match load_addr Mptr m fin with (* derefencing **fin *)
   | Some (Vptr b ofs) =>  
              match addr_ge str (b,ofs) with (* compare str and *fin *)
@@ -130,14 +132,14 @@ Definition asn_strtoimax_lim (str fin : addr) : option (asn_strtox_result_e*(opt
              | Some false => let dist := distance str (b,ofs) in
                             match load_addr Mint8signed m str with
                             | Some (Vint i) =>
-                              if (i == minus_char)
+                              if (i == minus_char)%int
                               then asn_strtoimax_lim_loop (str++) fin 0 Signed last_digit_max_minus (dist - 1)%nat m
-                              else if (i == plus_char)
+                              else if (i == plus_char)%int
                                    then
                                      if addr_ge (str++) (b,ofs)
                                      then Some (ASN_STRTOX_EXPECT_MORE, None, (Mem.storev Mptr m (vptr fin) (vptr (str++))))
-                                     else  asn_strtoimax_lim_loop (str++) fin 0 Unsigned last_digit_max_plus (dist - 1)%nat m
-                                   else asn_strtoimax_lim_loop str fin 0 Unsigned last_digit_max_plus dist m
+                                     else  asn_strtoimax_lim_loop (str++) fin 0 Unsigned last_digit_max (dist - 1)%nat m
+                                   else asn_strtoimax_lim_loop str fin 0 Unsigned last_digit_max dist m
                             | _ => None (* fail of memory load on str: wrong type or not enough permission *)
                             end
              | None => None (* error in pointer comparison *)
@@ -145,52 +147,15 @@ Definition asn_strtoimax_lim (str fin : addr) : option (asn_strtox_result_e*(opt
    | _ => None (* fail of pointer to fin *) 
   end.
 
-(* Useful lemmas about the spec *)
-(* Inversion lemmas *)
-Lemma strtoimax_loop_inv : forall n str fin outp m' value,
-    asn_strtoimax_lim_loop str fin value Signed last_digit_max_minus (S n) m =
-    Some (ASN_STRTOX_OK, outp, m') ->
-    exists i, asn_strtoimax_lim_loop (str ++) fin  (value * Int.repr 10 + (i - zero_char)) Signed last_digit_max_minus n m =
-    Some (ASN_STRTOX_OK, outp, m').
-Proof.
-  intros.
-  simpl in H.
-  break_if.
-  all: repeat break_match; try congruence; exists i; assumption.
-Qed.
-
-Lemma strtoimax_inv_mem : forall n str fin outp m' value, 
-  asn_strtoimax_lim_loop str fin value Signed last_digit_max_minus n m = Some (ASN_STRTOX_OK, outp, m') ->
-  forall i, (i < n)%nat -> exists v, load_addr Mint8signed m (add_addr str (Ptrofs.repr (Z.of_nat i))) = Some (Vint v) /\ is_digit v = true.
-Proof.
-  induction n.
-  - intros. nia.
-  - intros until value; intro H.
-    pose (strtoimax_loop_inv _ _ _ _ _ _ H) as S.
-    destruct S as [j S].
-    pose (IHn (str++) fin  outp _ (value * Int.repr 10 + (j - zero_char))  S) as N.
-    Admitted.
-
 Ltac exec_until_seq := 
      repeat  match goal with
             | [ |- exec_stmt _ _ _ _ (Ssequence _ _)  _ _ _ _ ] => idtac
             | _ => econstructor ; exec_until_seq
 
              end.
+(* Lemmas for each `asn_strtox_result_e` case *)
 
-Lemma loop_result : forall  (dist : nat) (str : addr) (fin : addr) (value : int) (s: signedness) (last_digit : int),
-    asn_strtoimax_lim_loop str fin value s last_digit dist m <> Some (ASN_STRTOX_ERROR_INVAL, None, None).
-Proof.
-  induction dist.
-  intros.
-  simpl.
-  congruence.
-  intros.
-  simpl.
-  repeat break_match.
-  repeat break_if.
-  all: try congruence.
-Qed.
+(* Case ASN_STRTOX_ERROR_INVAL *)
 
 Lemma asn_strtoimax_lim_ASN_STRTOX_ERROR_INVAL_correct : forall le str fin,
     
@@ -203,17 +168,23 @@ Lemma asn_strtoimax_lim_ASN_STRTOX_ERROR_INVAL_correct : forall le str fin,
 Proof.
   intros.
   unfold asn_strtoimax_lim in H.
-  
-  break_match.
-  break_match.
+   assert (forall dist str fin value s last_digit, asn_strtoimax_lim_loop str fin value s last_digit dist m <> Some (ASN_STRTOX_ERROR_INVAL, None, None)) as Loop.
+    { induction dist.
+      intros.
+      simpl.
+      congruence.
+      intros.
+      simpl.
+      repeat break_match.
+      repeat break_if.
+      all: try congruence. } 
+  repeat break_match.
   all: try congruence.
-  break_match.
   unfold addr_ge in Heqo0.
   destruct b0.
   unfold vptr in *.
   repeat break_let.
-   unfold addr_ge in Heqo0.
-   replace (asn_strtox_result_e_to_int ASN_STRTOX_ERROR_INVAL) with  (Int.repr (-2)).
+   replace (asn_strtox_result_e_to_int ASN_STRTOX_ERROR_INVAL) with  (Int.repr (-2)) by (cbv; auto).
   repeat eexists.
   intros Str Fin.
   exec_until_seq.
@@ -232,10 +203,6 @@ Proof.
   apply Str.
   1-4: try (cbv;congruence).
   apply PTree.gss.
-  simpl.
-  unfold sem_cmp.
-  simpl.
-  unfold cmp_ptr.
   assert (option_map Val.of_bool
     (if Archi.ptr64
      then Val.cmplu_bool (Mem.valid_pointer m) Cge (Vptr b0 i0) (Vptr b i)
@@ -244,16 +211,179 @@ Proof.
   unfold ptr_ge in Heqo0.
   assumption.
     eapply H0.
-    simpl.
     econstructor.
     repeat econstructor.
-    cbv; congruence.
-    cbv. auto.
-    repeat break_match.
-    all: try congruence.
-    all: pose (loop_result _ _ _ _ _ _ H).
-    all: contradiction.
+    all: congruence.
 Qed.
+
+(* Useful lemmas about the spec *)
+(* Inversion lemmas *)
+Lemma strtoimax_loop_inv : forall n str fin outp m' value,
+    asn_strtoimax_lim_loop str fin value Signed last_digit_max_minus (S n) m =
+    Some (ASN_STRTOX_OK, outp, m') ->
+    exists i, asn_strtoimax_lim_loop (str ++) fin  (value * Int64.repr 10 + int_to_int64 (i - zero_char)%int) Signed last_digit_max_minus n m =
+    Some (ASN_STRTOX_OK, outp, m').
+Proof.
+  intros.
+  simpl in H.
+  break_if.
+  all: repeat break_match; try congruence; exists i; assumption.
+Qed.
+
+Lemma strtoimax_inv_mem : forall n str fin outp m' value, 
+  asn_strtoimax_lim_loop str fin value Signed last_digit_max_minus n m = Some (ASN_STRTOX_OK, outp, m') ->
+  forall i, (i < n)%nat -> exists v, load_addr Mint8signed m (add_addr str (Ptrofs.repr (Z.of_nat i))) = Some (Vint v) /\ is_digit v = true.
+Proof.
+  induction n.
+  - intros. nia.
+  - intros until value; intro H.
+    pose (strtoimax_loop_inv _ _ _ _ _ _ H) as S.
+    destruct S as [j S].
+    pose (IHn (str++) fin  outp _ (value * Int64.repr 10 +  int_to_int64 (j - zero_char)%int)  S) as N.
+Admitted.
+
+(* case ASN_STRTOX_EXPECT_MORE: reading + or - and reaching *end *)
+
+Lemma asn_strtoimax_lim_ASN_STRTOX_EXPECT_MORE_correct : forall le str fin m', 
+    asn_strtoimax_lim str fin = Some (ASN_STRTOX_EXPECT_MORE, None, Some m') ->
+    exists t le', le!_str = Some (vptr str)  ->
+             le!_end = Some (vptr fin) ->
+             le! _last_digit_max = Some (Vlong last_digit_max) -> 
+      
+             exec_stmt ge e le m f_asn_strtoimax_lim.(fn_body) t le' m' (Out_return (Some (Vint (asn_strtox_result_e_to_int ASN_STRTOX_EXPECT_MORE), tint)))
+             /\ le'!_end = Some (vptr str).
+Proof.
+
+  replace (asn_strtox_result_e_to_int ASN_STRTOX_EXPECT_MORE) with (Int.repr (-1)) by (cbv; auto).
+  assert (forall dist str fin s last_digit v m',
+             asn_strtoimax_lim_loop str fin v s last_digit dist m <>  Some (ASN_STRTOX_EXPECT_MORE, None, Some m')) as Loop.
+    { induction dist.
+      intros.
+      simpl.
+      congruence.
+      intros.
+      simpl.
+      repeat break_match.
+      repeat break_if.
+      all: try congruence;
+       eapply IHdist.        }
+  intros until m'; intros Spec.
+    unfold vptr.
+      unfold asn_strtoimax_lim in Spec.  
+
+  repeat break_let.
+  repeat break_match.
+  all: try congruence.
+  
+  pose (Loop  (distance (b, i) (b1, i1) - 1)%nat  ((b, i) ++) (b0, i0) Signed last_digit_max_minus 0  m' ). congruence.
+
+  
+  repeat eexists.
+  exec_until_seq.
+   econstructor.
+   repeat econstructor.
+   econstructor.
+   repeat econstructor.
+   econstructor.
+   repeat econstructor.
+  repeat rewrite PTree.gso.
+  eapply H0.
+  1-3: cbv; congruence.
+  (* dereferencing double pointer *)
+  
+  apply Heqo.
+  repeat rewrite PTree.gso.
+  apply H.
+  1-4: cbv; congruence.
+  apply PTree.gss.
+  simpl.
+  assert (sem_cmp Cge (Vptr b i) (tptr tschar)  (Vptr b1 i1) (tptr tschar) m = Some Vfalse) by admit. (* follows from spec: TODO*)
+  apply H2.  
+  repeat econstructor.
+  repeat econstructor.
+  apply exec_Sseq_2.
+  repeat econstructor.
+  repeat rewrite PTree.gso.
+  apply H.
+  1-4: cbv; congruence.
+  apply Heqo1.
+  
+  replace  (Out_return (Some (Vint (Int.repr (-1)), tint))) with (outcome_switch  (Out_return (Some (Vint (Int.repr (-1)), tint)))).
+  repeat econstructor.
+  repeat rewrite PTree.gso.
+  eapply H.
+  1-5: cbv; congruence.
+  simpl in Heqo1.
+  simpl.
+  apply Heqo1.
+  repeat econstructor.
+  replace i2 with minus_char.
+  econstructor.
+  econstructor.
+    exec_until_seq.
+  (rewrite PTree.gso).
+  (rewrite PTree.gso).
+  apply PTree.gss.
+  1-2: cbv; try congruence.
+  1-2: 
+    repeat econstructor.
+  apply exec_Sseq_2.
+  econstructor.
+  repeat econstructor.
+  repeat  (rewrite PTree.gso).
+  apply H.
+  1-7: cbv; congruence.
+  unfold tlong.
+  unfold tint.
+  simpl.
+  econstructor.
+  repeat econstructor.
+  repeat  (rewrite PTree.gso).
+  apply H0.
+  1-8: cbv; congruence.
+  simpl in Heqo.
+  simpl.
+  apply Heqo.
+  (rewrite PTree.gso).
+  apply PTree.gss.
+  cbv; congruence.
+  apply PTree.gss.
+  simpl.
+  assert (sem_cmp Cge (Vptr b (i + Ptrofs.repr 1 * Ptrofs.of_ints (Int.repr 1))%ptrofs)
+                  (tptr tschar) (Vptr b1 i1) (tptr tschar) m = Some Vtrue) by admit.
+  apply H2.
+  repeat econstructor.
+  repeat econstructor.
+   repeat  (rewrite PTree.gso).
+  apply H0.
+  1-9: cbv; congruence.
+  (rewrite PTree.gso).
+  apply PTree.gss.
+  cbv; congruence.
+  repeat econstructor.
+  simpl.
+  assert ( Mem.store Mptr m b0 (Ptrofs.unsigned i0)
+    (Vptr b (i + Ptrofs.repr 1 * Ptrofs.of_ints (Int.repr 1))%ptrofs) = 
+           Some m') by admit.
+  apply H2.
+  cbv; congruence.
+  admit. (* spec *)
+  simpl. auto.
+  congruence.
+  admit. (* forgot intp! *)
+  admit. (* _end = _str ??? *)
+  
+
+  
+  
+  pose (Loop  (distance (b, i) (b1, i1) - 1)%nat  ((b, i) ++) (b0, i0) Unsigned last_digit_max 0  m' ).  congruence.
+  pose (Loop  (distance (b, i) (b1, i1))  ((b, i)) (b0, i0) Unsigned last_digit_max 0  m' ).  congruence.
+  
+ 
+Admitted.
+    
+
+(* Loop correctness cases *)
 
 Lemma asn_strtoimax_lim_loop_ASN_STRTOX_EXTRA_DATA_correct : forall dist le str fin value s last_digit,
     
@@ -261,15 +391,16 @@ Lemma asn_strtoimax_lim_loop_ASN_STRTOX_EXTRA_DATA_correct : forall dist le str 
     
      exists t le', le!_str = Some (vptr str)  ->
                    le!_end = Some (vptr fin) ->
-                   le!_value = Some (Vlong (Int64.repr (Int.unsigned value))) ->
+                   le!_value = Some (Vlong value) ->
               
-             exec_stmt ge e le m f_asn_strtoimax_lim_loop t le' m (Out_return (Some (Vint (asn_strtox_result_e_to_int ASN_STRTOX_EXTRA_DATA), tint))).
+                   exec_stmt ge e le m f_asn_strtoimax_lim_loop t le' m
+                             (Out_return (Some (Vint (asn_strtox_result_e_to_int ASN_STRTOX_EXTRA_DATA), tint))).
 Proof.
   induction dist.
   intros.
   simpl in H. congruence.
   intros.
-  simpl in H.
+  simpl in H.                           
   repeat break_match.
   all: try congruence.
   pose (IHdist le (str ++) fin (value * Int.repr 10 + (i - zero_char)) s
@@ -362,118 +493,5 @@ Proof.
 
 
 
-Lemma asn_strtoimax_lim_ASN_STRTOX_EXPECT_MORE_correct : forall le str fin value m', 
-    asn_strtoimax_lim str fin = Some (ASN_STRTOX_EXPECT_MORE, Some (value, Unsigned), Some m') ->
-    exists t le', le!_str = Some (vptr str)  ->
-             le!_end = Some (vptr fin) ->
-      
-             exec_stmt ge e le m f_asn_strtoimax_lim.(fn_body) t le' m' (Out_return (Some (Vint (asn_strtox_result_e_to_int ASN_STRTOX_EXPECT_MORE), tint)))
-             /\ le'!_intp = Some (Vint value)
-             /\ le'!_end = Some (vptr str).
-Proof.
-  replace (asn_strtox_result_e_to_int ASN_STRTOX_EXPECT_MORE) with (Int.repr (-1)) by admit.
-  intros until value; intros m' Spec.
-  unfold vptr.
-  repeat break_let.
-  unfold asn_strtoimax_lim in Spec.
-  repeat break_match.
-  all: try congruence.
-  repeat eexists.
-  exec_until_seq.
-   econstructor.
-   repeat econstructor.
-   econstructor.
-   repeat econstructor.
-   econstructor.
-   repeat econstructor.
-  repeat rewrite PTree.gso.
-  eapply H0.
-  1-3: cbv; congruence.
-  (* dereferencing double pointer *)
-  
-  apply Heqo.
-  repeat rewrite PTree.gso.
-  apply H.
-  1-4: cbv; congruence.
-  apply PTree.gss.
-  simpl.
-  assert (sem_cmp Cge (Vptr b i) (tptr tschar)  (Vptr b1 i1) (tptr tschar) m = Some Vfalse) by admit. (* follows from spec: TODO*)
-  apply H1.  
-  repeat econstructor.
-  repeat econstructor.
-  apply exec_Sseq_2.
-  repeat econstructor.
-  repeat rewrite PTree.gso.
-  apply H.
-  1-4: cbv; congruence.
-  apply Heqo1.
-  
-  replace  (Out_return (Some (Vint (Int.repr (-1)), tint))) with (outcome_switch  (Out_return (Some (Vint (Int.repr (-1)), tint)))).
-  repeat econstructor.
-  repeat rewrite PTree.gso.
-  eapply H.
-  1-5: cbv; congruence.
-  simpl in Heqo1.
-  simpl.
-  apply Heqo1.
-  repeat econstructor.
-  replace i2 with minus_char.
-  econstructor.
-  econstructor.
-    exec_until_seq.
-  
-  assert ((le! _last_digit_max) = Some (Vint last_digit_max_minus)) by admit. (* change to int64 *)
-  (rewrite PTree.gso).
-  (rewrite PTree.gso).
-  apply PTree.gss.
-  1-2: cbv; try congruence.
-  1-2: 
-    repeat econstructor.
-  apply exec_Sseq_2.
-  econstructor.
-  repeat econstructor.
-  repeat  (rewrite PTree.gso).
-  apply H.
-  1-7: cbv; congruence.
-  unfold tlong.
-  unfold tint.
-  simpl.
-  econstructor.
-  repeat econstructor.
-  repeat  (rewrite PTree.gso).
-  apply H0.
-  1-8: cbv; congruence.
-  simpl in Heqo.
-  simpl.
-  apply Heqo.
-  (rewrite PTree.gso).
-  apply PTree.gss.
-  cbv; congruence.
-  apply PTree.gss.
-  simpl.
-  assert (sem_cmp Cge (Vptr b (i + Ptrofs.repr 1 * Ptrofs.of_ints (Int.repr 1))%ptrofs)
-                  (tptr tschar) (Vptr b1 i1) (tptr tschar) m = Some Vtrue) by admit.
-  apply H1.
-  repeat econstructor.
-  repeat econstructor.
-   repeat  (rewrite PTree.gso).
-  apply H0.
-  1-9: cbv; congruence.
-  (rewrite PTree.gso).
-  apply PTree.gss.
-  cbv; congruence.
-  repeat econstructor.
-  simpl.
-  assert ( Mem.store Mptr m b0 (Ptrofs.unsigned i0)
-    (Vptr b (i + Ptrofs.repr 1 * Ptrofs.of_ints (Int.repr 1))%ptrofs) = 
-           Some m') by admit.
-  apply H1.
-  cbv; congruence.
-  admit. (* spec *)
-  simpl. auto.
-  congruence.
-  admit. (* forgot intp! *)
-  admit. (* _end = _str ??? *)
-Admitted.
-    
+
     
